## Describing sequence patterns by expressions
Let's represent a sequence of integers with a[0], a[1], a[2], ..., a[i]. If a sequence is such that for i > 1 we have a[i] = f(x, y, i) where x=a[i-2], y=a[i-1], and f is a function (expression involving i, x, or y), then the function describes the pattern of the sequence. In other words, the elements of the sequence from the third element onwards can be generated by the expression.

- **Example 1:** The sequence 0, 1, 2, 3, 4, 5, 6,... can be described by f(x, y, i) = i or f(x, y, i)=y+1 or f(x, y, i) = x + 2.

- **Example 2:** The sequence 1, 4, 9, 16, 25,... can be described by f(x, y, i) = (i+1)*(1+i).

- **Example 3:** The sequence 0, 1, 1, 2, 3, 5, 8, 13, ..., the Fibonacci sequence, can be described by f(x, y, i) = x + y.